Add a conference tutorial (#299)
* Start working on the tutorial

* Improve scalar_tac, progress, introduce delaboration for scalars and work on the tutorial

* Remove List.len and use List.length instead

* Start working on a bignum library for the tutorial

* Add some missing changes

* Add support for scalar negation

* Add missing files for the tutorial

* Update the charon pin

* Add alloc.vec.Vec.resize in the Lean library

* Update the code for the bignums

* Update progress to use simp on the preconditions

* Add definition for overflowing_add to the Lean library

* Make the trait implementations reducible

* Regenerate the files

* Update progress to better control the instantiation of meta-variables

If there are meta-variables in a precondition, progress will apply an assumption
(which instantiates the meta-variables) only if there is a unique assumption
matching the precondition.

* Improve progress a bit

* Fix issues in Primitives.{v,fst}

* Make good progress on the tutorial

* Make minor modifications to scalar_tac

* Fix the proofs of the hashmap

* Regenerate the files

* Start working on a forward saturation function

* Make good progress on the forward saturation function

* Add a missing file

* Add tactics to normalize scalar goals

* Improve the saturation tactic to allow erasing rules and using local rules

* Print more informative error messages when saturation patterns are not valid

* Drastically improve scalar_tac

* Update the proofs in the tutorial

* Move and update lemmas

* Start replacing the List functions which use integers

* Finish replacing the list functions in the Lean library

* Start updating the examples

* Update the proofs of the hashmap

* Update the BaseTutorial

* Reduce the proof time of the hashmap and the AVL

* Update the tutorial

* Make minor modifications

* Introduce a dcases tactic and update the tutorial

* Fix an issue with the Primitives.fst file

* Finish the tutorial

* Fix an issue with the tutorial

* Fix an issue with Primitives.v

* Make minor modifications

* Make more minor modifications

compiler/ExtractTypes.ml
@@ -94,7 +94,7 @@ let extract_unop (span : Meta.span) (extract_expr : bool -> texpression -> unit)
     (fmt : F.formatter) (inside : bool) (unop : unop) (arg : texpression) : unit
     =
   match unop with
-  | Not | Neg _ ->
+  | Not _ | Neg _ ->
       let unop = unop_name unop in
       if inside then F.pp_print_string fmt "(";
       F.pp_print_string fmt unop;
