backends/lean/Base/Saturate/Tactic.lean
@@ -1,0 +1,216 @@
+import Base.Saturate.Attribute
+
+open Lean Lean.Meta Lean.Elab Lean.Elab.Term Lean.Elab.Tactic
+open Utils Extensions
+
+namespace Saturate
+
+open Attribute
+
+/-- Find all the lemmas which match an expression.
+
+    - `dtrees`: the discrimination trees (the sets of rules in which to match)
+    - `boundVars`: if an instantiation of a theorem contains a bound variable, we ignore
+      it (because we couldn't introduce the instantiated theorem it in the environment)
+    - `matched`: the theorems to apply (the set of theorem name and list of arguments)
+
+    We return the set of: (theroem name, list of arguments)
+ -/
+def matchExpr (nameToRule : NameMap Rule) (dtrees : Array (DiscrTree Rule))
+  (boundVars : HashSet FVarId)
+  (matched : HashSet (Name × List Expr)) (e : Expr) :
+  MetaM (HashSet (Name × List Expr)) := do
+  trace[Saturate] "Matching: {e}"
+  dtrees.foldlM (fun matched dtree => do
+    let config : WhnfCoreConfig := {}
+    let exprs ← dtree.getMatch e config
+    trace[Saturate] "Potential matches: {exprs}"
+    -- Check each expression
+    (exprs.foldlM fun matched rule => do
+      -- Check if the theorem is still active
+      if let some activeRule := nameToRule.find? rule.thName then do
+        -- Check that the patterns are the same
+        if activeRule.numBinders = rule.numBinders ∧ (← isDefEq activeRule.pattern rule.pattern) then
+          -- Introduce meta-variables for the universes
+          let info ← getConstInfo rule.thName
+          let mvarLevels ← mkFreshLevelMVarsFor info
+          let pat := rule.pattern.instantiateLevelParams info.levelParams mvarLevels
+          -- Strip the binders, introduce meta-variables at the same time, and match
+          let (mvars, _, pat) ← lambdaMetaTelescope pat (some rule.numBinders)
+          if ← isDefEq pat e then
+            -- It matched! Check the variables which appear in the arguments
+            let (args, allFVars) ← mvars.foldrM (fun arg (args, hs) => do
+                let arg ← instantiateMVars arg
+                let hs ← getFVarIds arg hs
+                pure (arg :: args, hs)
+              ) ([], HashSet.empty)
+            if boundVars.all (fun fvar => ¬ allFVars.contains fvar) then
+              -- Ok: save the theorem
+              trace[Saturate] "Matched with: {rule.thName} {args}"
+              pure (matched.insert (rule.thName, args))
+            else
+              -- Ignore
+              trace[Saturate] "Didn't match"
+              pure matched
+          else
+            -- Didn't match, leave the set of matches unchanged
+            trace[Saturate] "Didn't match"
+            pure matched
+        else
+          -- The rule is not active
+          trace[Saturate] "The rule is not active"
+          pure matched
+      else
+        -- The rule is not active
+        trace[Saturate] "The rule is not active"
+        pure matched) matched
+  ) matched
+
+/- Recursively explore a term -/
+private partial def visit (depth : Nat) (nameToRule : NameMap Rule)
+  (dtrees : Array (DiscrTree Rule))
+  (boundVars : HashSet FVarId)
+  (matched : HashSet (Name × List Expr))
+  (e : Expr) : MetaM (HashSet (Name × List Expr)) := do
+  trace[Saturate] "Visiting {e}"
+  -- Match
+  let matched ← matchExpr nameToRule dtrees boundVars matched e
+  -- Recurse
+  let visitBinders
+    (depth : Nat)
+    (boundVars : HashSet FVarId) (matched : HashSet (Name × List Expr)) (xs: Array Expr) :
+    MetaM (HashSet FVarId × (HashSet (Name × List Expr))) := do
+    -- Visit the type of the binders, as well as the bodies
+    xs.foldlM (fun (boundVars, matched) x => do
+      let fvarId := x.fvarId!
+      let localDecl ← fvarId.getDecl
+      let boundVars := boundVars.insert fvarId
+      let matched ← visit (depth + 1) nameToRule dtrees boundVars matched localDecl.type
+      let matched ←
+        match localDecl.value? with
+        | none => pure matched
+        | some v => visit (depth + 1) nameToRule dtrees boundVars matched v
+      pure (boundVars, matched)
+      ) (boundVars, matched)
+  let e := e.consumeMData
+  match e with
+  | .bvar _
+  | .fvar _
+  | .mvar _
+  | .sort _
+  | .lit _
+  | .const _ _ =>
+    trace[Saturate] "Stop: bvar, fvar, etc."
+    pure matched
+  | .app .. => do e.withApp fun f args => do
+    trace[Saturate] ".app"
+    -- Visit the args
+    let matched ← args.foldlM (fun matched arg => visit (depth + 1) nameToRule dtrees boundVars matched arg) matched
+    -- Visit the app
+    visit (depth + 1) nameToRule dtrees boundVars matched f
+  | .lam .. =>
+    trace[Saturate] ".lam"
+    lambdaLetTelescope e fun xs b => do
+      let (boundVars, matched) ← visitBinders (depth + 1) boundVars matched xs
+      visit (depth + 1) nameToRule dtrees boundVars matched b
+  | .forallE .. => do
+    trace[Saturate] ".forallE"
+    forallTelescope e fun xs b => do
+      let (boundVars, matched) ← visitBinders (depth + 1) boundVars matched xs
+      visit (depth + 1) nameToRule dtrees boundVars matched b
+  | .letE .. => do
+    trace[Saturate] ".letE"
+    lambdaLetTelescope e fun xs b => do
+      let (boundVars, matched) ← visitBinders (depth + 1) boundVars matched xs
+      visit (depth + 1) nameToRule dtrees boundVars matched b
+  | .mdata _ b => do
+    trace[Saturate] ".mdata"
+    visit (depth + 1) nameToRule dtrees boundVars matched b
+  | .proj _ _ b => do
+    trace[Saturate] ".proj"
+    visit (depth + 1) nameToRule dtrees boundVars matched b
+
+/- The saturation tactic itself -/
+def evalSaturate (sets : List Name) : TacticM Unit := do
+  Tactic.withMainContext do
+  trace[Saturate] "sets: {sets}"
+  -- Retrieve the rule sets
+  let s := Saturate.Attribute.saturateAttr.ext.getState (← getEnv)
+  let dtrees := Array.mk (sets.filterMap (fun set => s.rules.find? set))
+  -- Get the local context
+  let ctx ← Lean.MonadLCtx.getLCtx
+  -- Explore the declarations
+  let decls ← ctx.getDecls
+  let matched ← decls.foldlM (fun matched (decl : LocalDecl) => do
+    trace[Saturate] "Exploring local decl: {decl.userName}"
+    /- We explore both the type, the expresion and the body (if there is) -/
+    let matched ← visit 0 s.nameToRule dtrees HashSet.empty matched decl.type
+    let matched ← visit 0 s.nameToRule dtrees HashSet.empty matched decl.toExpr
+    match decl.value? with
+    | none => pure matched
+    | some value => visit 0 s.nameToRule dtrees HashSet.empty matched value) HashSet.empty
+  -- Explore the goal
+  trace[Saturate] "Exploring the goal"
+  let matched ← visit 0 s.nameToRule dtrees HashSet.empty matched (← Tactic.getMainTarget)
+  -- Introduce the theorems in the context
+  for (thName, args) in matched do
+    let th ← mkAppOptM thName (args.map some).toArray
+    let thTy ← inferType th
+    let _ ← Utils.addDeclTac (.str .anonymous "_") th thTy (asLet := false)
+
+elab "aeneas_saturate" : tactic =>
+  evalSaturate [`Aeneas.ScalarTac]
+
+section Test
+  local elab "aeneas_saturate_test" : tactic =>
+    evalSaturate [`Aeneas.Test]
+
+  set_option trace.Saturate.attribute false
+  @[aeneas_saturate (set := Aeneas.Test) (pattern := l.length)]
+  theorem rule1 (α : Type u) (l : List α) : l.length ≥ 0 := by simp
+
+  set_option trace.Saturate false
+
+  theorem test1 {α : Type v} (l0 l1 l2 l3 l4 l5 : List α)
+    (_ : ∀ (l : List α), l.length ≤ l3.length) :
+    let _k := l4.length
+    let _g := fun (l : List α) => l.length + l5.length
+    (l0 ++ l1 ++ l2).length = l0.length + l1.length + l2.length := by
+    aeneas_saturate_test
+    simp [Nat.add_assoc]
+
+  namespace Test
+    set_option trace.Saturate.attribute false
+    @[local aeneas_saturate (set := Aeneas.Test) (pattern := l.length)]
+    theorem rule2 (α : Type u) (l : List α) : 0 ≤ l.length := by simp
+
+    theorem test1 {α : Type v} (l0 l1 l2 l3 l4 l5 : List α)
+      (_ : ∀ (l : List α), l.length ≤ l3.length) :
+      let _k := l4.length
+      let _g := fun (l : List α) => l.length + l5.length
+      (l0 ++ l1 ++ l2).length = l0.length + l1.length + l2.length := by
+      aeneas_saturate_test
+      simp [Nat.add_assoc]
+
+    attribute [- aeneas_saturate] rule2
+
+    theorem test2 {α : Type v} (l0 l1 l2 l3 l4 l5 : List α)
+      (_ : ∀ (l : List α), l.length ≤ l3.length) :
+      let _k := l4.length
+      let _g := fun (l : List α) => l.length + l5.length
+      (l0 ++ l1 ++ l2).length = l0.length + l1.length + l2.length := by
+      aeneas_saturate_test
+      simp [Nat.add_assoc]
+  end Test
+
+  theorem test3 {α : Type v} (l0 l1 l2 l3 l4 l5 : List α)
+    (_ : ∀ (l : List α), l.length ≤ l3.length) :
+    let _k := l4.length
+    let _g := fun (l : List α) => l.length + l5.length
+    (l0 ++ l1 ++ l2).length = l0.length + l1.length + l2.length := by
+    aeneas_saturate_test
+    simp [Nat.add_assoc]
+
+end Test
+
+end Saturate
