tests/lean/External/Funs.lean
@@ -13,6 +13,7 @@ namespace external
 /- Trait implementation: [core::marker::{core::marker::Copy for u32}#40]
    Source: '/rustc/library/core/src/marker.rs', lines 48:25-48:62
    Name pattern: core::marker::Copy<u32> -/
+@[reducible]
 def core.marker.CopyU32 : core.marker.Copy U32 := {
   cloneCloneInst := core.clone.CloneU32
 }
